SEARrecty.sml
@@ -2,7 +2,16 @@
 
 val InjN_def = proved_th $
 e0
-(cheat)
+(strip_tac >> irule
+ (P2fun_uex |> qspecl [‘N’,‘Pow(N * A)’] 
+ |> fVar_sInst_th “P(n0:mem(N),na:mem(Pow(N * A)))”
+    “(!n:mem(N) a:mem(A).IN(Pair(n,a),na) <=> n = n0)”) >>
+ strip_tac >> accept_tac
+ (IN_def_P |> qspecl [‘N * A’] 
+ |> fVar_sInst_th “P(na:mem(N * A))” “Fst(na:mem(N * A)) = x”
+ |> conv_rule (depth_fconv no_conv forall_cross_fconv)
+ |> rewr_rule[Pair_def'])
+)
 (form_goal “!A. ?!injN:N -> Pow(N * A).
  !n0. (!n a.IN(Pair(n,a),App(injN,n0)) <=> n = n0)”)
 |> spec_all |> uex2ex_rule |> qSKOLEM "InjN" [‘A’] |> gen_all 
@@ -10,7 +19,15 @@ e0
 
 val InjA_def = proved_th $
 e0
-(cheat)
+(strip_tac >> irule
+ (P2fun_uex |> qspecl [‘A’,‘Pow(N * A)’] 
+ |> fVar_sInst_th “P(a0:mem(A),na:mem(Pow(N * A)))”
+    “(!n:mem(N) a:mem(A).IN(Pair(n,a),na) <=> a = a0)”) >>
+ strip_tac >> accept_tac
+ (IN_def_P |> qspecl [‘N * A’] 
+ |> fVar_sInst_th “P(na:mem(N * A))” “Snd(na:mem(N * A)) = x”
+ |> conv_rule (depth_fconv no_conv forall_cross_fconv)
+ |> rewr_rule[Pair_def']))
 (form_goal “!A. ?!injA:A -> Pow(N * A).
  !a0. (!n a.IN(Pair(n,a),App(injA,a0)) <=> a = a0)”)
 |> spec_all |> uex2ex_rule |> qSKOLEM "InjA" [‘A’] |> gen_all 
@@ -18,48 +35,145 @@ e0
 val Even_def = qdefine_psym("Even",[‘n:mem(N)’]) ‘∃n0. n = Mul(Suc(Suc(O)),n0)’
 val Odd_def = qdefine_psym("Odd",[‘n:mem(N)’]) ‘~Even(n)’
 
-(*pretend we have div*)
-val DIV2_def = proved_th $
-e0
-cheat
-(form_goal “∃!f:N ->N. (∀n.Even(n) ⇔ App(f,n) = O) &
- (∀n. Odd(n) ⇔ App(f,n) = Suc(O)) ”)
-|> uex2ex_rule |> qSKOLEM "DIV2" []
 
-val Div_def = qdefine_fsym("Div2",[‘n:mem(N)’]) ‘App(DIV2,n)’
-
-                          
-val InjUU_def = proved_th $
-e0
-cheat
-(form_goal “∀A.∃!f:Pow(N * A) * Pow(N * A) -> Pow(N * A).
- ∀u1 u2. ∀n a. IN(Pair(n,a),App(f,Pair(u1,u2))) ⇔ 
-  ((Even(n) & IN(Pair(Div2(n),a),u1)) | 
-   (Odd(n) & IN(Pair(Div2(n),a),u2)))”)
-|> spec_all |> uex2ex_rule |> qSKOLEM "InjUU" [‘A’]
-
-val injN_def = qdefine_fsym("injN",[‘A’,‘n:mem(N)’]) ‘App(InjN(A),n)’
-val injA_def = qdefine_fsym("injA",[‘a:mem(A)’]) ‘App(InjA(A),a)’ 
-val injUU_def = 
-    qdefine_fsym("injUU",[‘u1:mem(Pow(N * A))’,‘u2:mem(Pow(N * A))’]) 
-                ‘App(InjUU(A),Pair(u1,u2))’ 
-
+(*pretend div2 is defined*)
+val Div2_def = qdefine_fsym("Div2",[‘n:mem(N)’]) ‘n’
 
 
 val num1_def = qdefine_fsym("num1",[]) ‘Suc(O)’
 val num2_def = qdefine_fsym("num2",[]) ‘Suc(num1)’
 val num3_def = qdefine_fsym("num3",[]) ‘Suc(num2)’
 val num4_def = qdefine_fsym("num4",[]) ‘Suc(num3)’
+                          
+val InjUU_def = proved_th $
+e0
+(strip_tac >> irule
+ (P2fun_uex |> qspecl [‘Pow(N * A) * Pow(N * A)’,‘Pow(N * A)’] 
+ |> fVar_sInst_th “P(u12:mem(Pow(N * A) * Pow(N * A)), s:mem(Pow(N * A)))”
+    “∀n a. IN(Pair(n,a),s:mem(Pow(N * A))) ⇔ 
+    ((Even(n) & IN(Pair(Div2(n),a),Fst(u12))) | 
+     (Odd(n) & IN(Pair(Div2(n),a),Snd(u12))))”
+ |> conv_rule (depth_fconv no_conv forall_cross_fconv)
+ |> rewr_rule[Pair_def']) >>
+ rpt strip_tac >> accept_tac
+ (IN_def_P |> qspecl [‘N * A’]
+ |> fVar_sInst_th “P(na:mem(N * A))”
+ “(Even(Fst(na)) & IN(Pair(Div2(Fst(na)),Snd(na)),a:mem(Pow(N * A)))) | 
+ (Odd(Fst(na)) & IN(Pair(Div2(Fst(na)),Snd(na)),b))”
+ |> conv_rule (depth_fconv no_conv forall_cross_fconv)
+ |> rewr_rule[Pair_def']))
+(form_goal “∀A.∃!f:Pow(N * A) * Pow(N * A) -> Pow(N * A).
+ ∀u1 u2. ∀n a. IN(Pair(n,a),App(f,Pair(u1,u2))) ⇔ 
+  ((Even(n) & IN(Pair(Div2(n),a),u1)) | 
+   (Odd(n) & IN(Pair(Div2(n),a),u2)))”)
+|> spec_all |> uex2ex_rule |> qSKOLEM "InjUU" [‘A’]
+
+val injUU_def = 
+    qdefine_fsym("injUU",[‘u1:mem(Pow(N * A))’,‘u2:mem(Pow(N * A))’]) 
+                ‘App(InjUU(A),Pair(u1,u2))’ 
+
+val Even_not_Odd = prove_store("Even_not_Odd",
+e0
+cheat
+(form_goal “!n. Even(n) <=> ~Odd(n)”));
+
+
+
+val Odd_not_Even = prove_store("Odd_not_Even",
+e0
+cheat
+(form_goal “!n. Odd(n) <=> ~Even(n)”));
+
+
+val injUU_char = prove_store("injUU_char",
+e0
+(rpt strip_tac (* 2 *)
+ >-- (rw[injUU_def,InjUU_def] >> arw[Odd_not_Even]) >> 
+ rw[injUU_def,InjUU_def] >> arw[Even_not_Odd])
+(form_goal “
+ (!n. Even(n) ==> (!A u1:mem(Pow(N * A)) u2 a. IN(Pair(n,a),injUU(u1,u2)) <=> IN(Pair(Div2(n),a),u1))) & 
+ (!n. Odd(n) ==> (!A u1:mem(Pow(N * A)) u2 a. IN(Pair(n,a),injUU(u1,u2)) <=> IN(Pair(Div2(n),a),u2)))”));
+
+val injUU_Even = injUU_char |> conjE1
+                            
+
+val InjUU_Inj = prove_store("InjUU_Inj",
+e0
+(strip_tac >> rw[Inj_def] >> rpt strip_tac >>
+ ccontra_tac >>
+ qsuff_tac ‘~(App(InjUU(A), x1) = App(InjUU(A), x2))’
+ >-- arw[] >>
+ last_x_assum (K all_tac) >>
+ qsspecl_then [‘x1’] (x_choosel_then ["u1","u2"] assume_tac) Pair_has_comp>>
+ qsspecl_then [‘x2’] (x_choosel_then ["u3","u4"] assume_tac) Pair_has_comp>>
+ fs[] >> fs[Pair_eq_eq] >> rw[GSYM injUU_def] >> 
+ qby_tac ‘~(u1 = u3) | ~(u2 = u4)’ >-- cheat >>
+ pop_assum strip_assume_tac >>
+ last_x_assum (K all_tac) (* 2 *)
+ >-- (fs[GSYM IN_EXT_iff] >> 
+     qby_tac ‘(?n a. IN(Pair(n,a),u1) & ~(IN(Pair(n,a),u3))) | 
+              (?n a. IN(Pair(n,a),u3) & ~(IN(Pair(n,a),u1)))’
+     >-- cheat >> pop_assum strip_assume_tac (* 2 *)
+     >-- (qsuff_tac
+         ‘?n a. IN(Pair(n,a),injUU(u1,u2)) & ~IN(Pair(n,a),injUU(u3,u4))’
+         >-- cheat >>
+         qexistsl_tac [‘Mul(num2,n)’,‘a’] >>
+         qby_tac ‘Even(Mul(num2,n))’ >-- cheat >>
+         drule injUU_Even >> arw[] >>
+         qby_tac ‘Div2(Mul(num2, n)) = n’ >-- cheat >> arw[])
+     >-- cheat (*same*)) >>
+ cheat)
+(form_goal “!A. Inj(InjUU(A))”));
+
+val injN_def = qdefine_fsym("injN",[‘A’,‘n:mem(N)’]) ‘App(InjN(A),n)’
+val injA_def = qdefine_fsym("injA",[‘a:mem(A)’]) ‘App(InjA(A),a)’ 
+
+
+
+
 
 (*FALSE *)
 val F0_def = qdefine_fsym("F0",[‘A’]) ‘injN(A,O)’
 
+val InjA_Inj = prove_store("InjA_Inj",
+e0
+(strip_tac >> rw[Inj_def] >> rw[GSYM IN_EXT_iff] >> 
+ fconv_tac (depth_fconv no_conv forall_cross_fconv) >>
+ rw[InjA_def] >> rpt strip_tac >>
+ first_x_assum (qspecl_then [‘O’,‘x1’] assume_tac) >> fs[])
+(form_goal “!A. Inj(InjA(A))”));
+
 val VAR0_def = qdefine_fsym("VAR0",[‘A’]) ‘InjUU(A) o Pa(El(injN(A,num1)) o To1(A),InjA(A))’
+
+val Pa_Inj = prove_store("Pa_Inj",
+e0
+(rpt strip_tac >> rw[Inj_def] >> rw[App_Pa_Pair] >> rw[Pair_eq_eq] >>
+ fs[Inj_def] >> rpt strip_tac >> first_x_assum irule >> arw[])
+(form_goal “!X A f:X->A. Inj(f) ==> !B g:X->B. Inj(Pa(g,f))”));
+
+val o_Inj_Inj = prove_store("o_Inj_Inj",
+e0
+cheat
+(form_goal “!A B f:A->B. Inj(f) ==> !C g:B->C. Inj(g) ==> Inj(g o f)”));
+
+val VAR0_Inj = prove_store("VAR0_Inj",
+e0
+(rw[VAR0_def] >> strip_tac >> irule o_Inj_Inj >>
+ rw[InjUU_Inj] >> irule Pa_Inj >> rw[InjA_Inj])
+(form_goal “!A.Inj(VAR0(A))”));
 
 val Var0_def = qdefine_fsym("Var0",[‘a:mem(A)’]) ‘App(VAR0(A),a)’
 
 val NEG0_def = qdefine_fsym("NEG0",[‘A’]) ‘InjUU(A) o 
 Pa(El(injN(A,num2)) o To1(Pow(N * A)),Id(Pow(N * A)))’
+
+
+val NEG0_Inj = prove_store("NEG0_Inj",
+e0
+(rw[NEG0_def] >> strip_tac >> irule o_Inj_Inj >>
+ rw[InjUU_Inj] >> irule Pa_Inj >> rw[Id_Inj])
+(form_goal “!A.Inj(NEG0(A))”));
+
 
 
 val Neg0_def = qdefine_fsym("Neg0",[‘f0:mem(Pow(N * A))’]) ‘App(NEG0(A),f0)’
@@ -68,16 +182,34 @@ val Neg0_def = qdefine_fsym("Neg0",[‘f0:mem(Pow(N * A))’]) ‘App(NEG0(A),f0
 val DISJ0_def = qdefine_fsym("DISJ0",[‘A’]) ‘InjUU(A) o 
 Pa(El(injN(A,num3)) o To1(Pow(N * A) * Pow(N * A)),InjUU(A))’
 
+
+val DISJ0_Inj = prove_store("DISJ0_Inj",
+e0
+(rw[DISJ0_def] >> strip_tac >> irule o_Inj_Inj >>
+ rw[InjUU_Inj] >> irule Pa_Inj >> rw[InjUU_Inj])
+(form_goal “!A.Inj(DISJ0(A))”));
+
+
 val Disj0_def = qdefine_fsym("Disj0",[‘f1:mem(Pow(N * A))’,‘f2:mem(Pow(N * A))’]) ‘App(DISJ0(A),Pair(f1,f2))’
 
 val DIAM0_def = qdefine_fsym("DIAM0",[‘A’])
 ‘InjUU(A) o 
 Pa(El(injN(A,num4)) o To1(Pow(N * A)),Id(Pow(N * A)))’
 
+
+
+val DIAM0_Inj = prove_store("DIAM0_Inj",
+e0
+(rw[DIAM0_def] >> strip_tac >> irule o_Inj_Inj >>
+ rw[InjUU_Inj] >> irule Pa_Inj >> rw[Id_Inj])
+(form_goal “!A.Inj(DIAM0(A))”));
+
+
 val Diam0_def = qdefine_fsym("Diam0",[‘f0:mem(Pow(N * A))’]) ‘App(DIAM0(A),f0)’
 
 
-
+(*How to automatically prove the constructors mutually disjoint?
+  *)
 val f = 
  “(nas = F0 ==> IN(nas,isfms)) &
   (!p:mem(A). nas = Var0(p) ⇒ IN(nas,isfms)) &
@@ -153,16 +285,6 @@ e0
  “!A p:mem(A). isfm(Var0(p))”)); 
 
 val isfm_clauses = isfm_rules |> rewr_rule[GSYM isfm_def]
-
-
-
-
-
-val isL_Ins = isL_rules |> spec_all |> conjE2 
-                        |> rewr_rule[GSYM isL_def]
-                        |> spec_all |> undisch 
-                        |> gen_all |> disch_all
-                        |> gen_all |> store_as "isL_Ins";
 
 
 val form_def = Thm_2_4  |> qspecl [‘Pow(N * A)’]
@@ -469,6 +591,7 @@ cheat
  (!f1 f2 f:mem(form(A)). ~(Disj(f1,f2) = Neg(f)))”));
 
 
+
 val Var_eq_eq = prove_store("Var_eq_eq",
 e0
 (cheat)
@@ -611,58 +734,16 @@ e0
      App(dmf,App(fmrec(x0,vf,nf,djf,dmf),f))) ”));
 
 
-val r2f_def = proved_th $
-e0
-cheat
-(form_goal “!R:A~>B. ?!f:A * B -> 1+1.
- !a b. App(f,Pair(a,b)) = App(i2(1,1),dot)  <=> Holds(R,a,b)”)
-|> spec_all |> uex2ex_rule |> qSKOLEM "r2f" [‘R’] |> gen_all
+
+val Vof_def = qdefine_fsym("Vof",[‘M:mem(Pow(W * W) * Exp(W,Pow(A)))’])
+‘tof(Snd(M))’ |> gen_all
 
 
-val true_def = qdefine_fsym("true",[]) ‘App(i2(1,1),dot)’
-
-val false_def = qdefine_fsym("false",[]) ‘App(i1(1,1),dot)’
-
-val tv_eq_true = prove_store("tv_eq_true",
-e0
-(cheat)
-(form_goal “!tv1 tv2. tv1 = tv2 <=>
- (tv1 = true <=> tv2 = true)”));
-
-val OR_def = proved_th $
-e0
-(cheat)
-(form_goal “?f:(1+1) * (1+1) -> 1+1. 
- App(f,Pair(true,true)) = true & 
- App(f,Pair(true,false)) = true &
- App(f,Pair(false,true)) = true &
- App(f,Pair(false,false)) = false”)
-|> qSKOLEM "OR" [] 
+val Rof_def = qdefine_fsym("Rof",[‘M:mem(Pow(W * W) * Exp(W,Pow(A)))’])
+‘Fst(M)’ |> gen_all
 
 
-val NOT_def = proved_th $
-e0
-(cheat)
-(form_goal “?f:1+1 -> 1+1. 
-App(f,true) = false & App(f,false) = true”)
-|> qSKOLEM "NOT" [] 
-
-
-
-val f2r_def = proved_th $
-e0
-cheat
-(form_goal “!A B f:A * B -> 1+1.?!R:A~>B.
- !a b. Holds(R,a,b) <=> App(f,Pair(a,b)) = true”)
-|> spec_all |> uex2ex_rule |> qSKOLEM "f2r" [‘f’] |> gen_all
-
-
-val ss2f = proved_th $
-e0
-(cheat)
-(form_goal “!A s:mem(Pow(A)).?!f:A -> 1+1.
- !a. App(f,a) = true <=> IN(a,s)”)
-|> spec_all |> uex2ex_rule |> qSKOLEM "ss2f" [‘s’]
+val Rm_def = qdefine_psym("Rm",[‘M:mem(Pow(W * W) * Exp(W,Pow(A)))’,‘w1:mem(W)’,‘w2:mem(W)’]) ‘IN(Pair(w1,w2),Rof(M))’;
 
 (*Holds at*)
 val HAT_def = proved_th $
@@ -673,7 +754,48 @@ cheat
 |> spec_all |> uex2ex_rule |> qSKOLEM "HAT" [‘M’]
 
 
-val Rm_def = qdefine_psym("Rm",[‘M:mem(Pow(W * W) * Exp(W,Pow(A)))’,‘w1:mem(W)’,‘w2:mem(W)’]) ‘IN(Pair(w1,w2),Rof(M))’;
+val INTER_def = proved_th $ 
+e0
+cheat
+(form_goal “!A. ?f:Pow(A) * Pow(A) -> Pow(A).
+ !s1 s2 a. IN(a,App(f,Pair(s1,s2))) <=> IN(a,s1) & IN(a,s2)”)
+|> spec_all |> qSKOLEM "INTER" [‘A’]
+
+val Inter_def = qdefine_fsym("Inter",[‘s1:mem(Pow(A))’,‘s2:mem(Pow(A))’])
+‘App(INTER(A),Pair(s1,s2))’
+
+
+
+val UNION_def = proved_th $ 
+e0
+cheat
+(form_goal “!A. ?f:Pow(A) * Pow(A) -> Pow(A).
+ !s1 s2 a. IN(a,App(f,Pair(s1,s2))) <=> IN(a,s1) | IN(a,s2)”)
+|> spec_all |> qSKOLEM "UNION" [‘A’]
+
+val IN_Inter = prove_store("IN_Inter",
+e0
+cheat
+(form_goal “!A s1 s2 a. IN(a:mem(A),Inter(s1,s2)) <=> IN(a,s1) & IN(a,s2)”));
+
+val EMPTY_def = qdefine_psym("EMPTY",[‘A’])
+‘!x:mem(A).F’
+
+val COMPL_def = proved_th $ 
+e0
+cheat
+(form_goal “!A. ?f:Pow(A) -> Pow(A).
+ !s a. IN(a,App(f,s)) <=> ~IN(a,s)”)
+|> spec_all |> qSKOLEM "COMPL" [‘A’]
+
+val Compl_def = qdefine_fsym("Compl",[‘s:mem(Pow(A))’])
+‘App(COMPL(A),s)’
+
+val IN_Compl = prove_store("IN_Compl",
+e0
+cheat
+(form_goal “!A s a. IN(a:mem(A),Compl(s)) <=> ~IN(a,s)”));
+
 
 val satis_dmf = proved_th $
 e0
@@ -797,6 +919,16 @@ e0
 (rw[Top_def,satis_def,satis_Bot])
 (form_goal “!A M w:mem(W). satis(M,w,Top(A))”));
 
+
+val Sim_def = qdefine_psym("Sim",[‘R:W1~>W2’,‘M1:mem(Pow(W1 * W1) * Exp(W1,Pow(A)))’,‘M2:mem(Pow(W2 * W2) * Exp(W2,Pow(A)))’]) 
+‘!w1 w2.Holds(R,w1,w2) ==>
+ (!p.IN(p,App(Vof(M1),w1)) ==> IN(p,App(Vof(M2),w2))) & 
+ (!v. Rm(M1,w1,v) ==> ?v'. Holds(R,v,v') & Rm(M2,w2,v'))’
+
+val PUS_def = qdefine_psym("PUS",[‘f:mem(form(A))’])
+‘!W1 W2 R:W1~>W2 M1:mem(Pow(W1 * W1) * Exp(W1,Pow(A))) M2. Sim(R,M1,M2) ==>
+ !w1 w2. Holds(R,w1,w2) ==> satis(M1,w1,f) ==> satis(M2,w2,f)’
+
 val PUS_Var = prove_store("PUS_Var",
 e0
 (rpt strip_tac >> rw[PUS_def,satis_def] >>
@@ -841,6 +973,9 @@ e0
 (form_goal “!A f:mem(form(A)). PE(f) ==> PUS(f)”));
 
 
+val EQV_def = qdefine_psym("EQV",[‘f1:mem(form(A))’,‘f2:mem(form(A))’])
+ ‘!W M w:mem(W). satis(M,w,f1) <=> satis(M,w,f2)’
+
 
 val Thm_6_25_r2l = prove_store("Thm_6_25_r2l",
 e0
@@ -848,42 +983,6 @@ e0
  fs[PUS_def] >> fs[EQV_def])
 (form_goal “!A f f0:mem(form(A)). PE(f0) & EQV(f,f0) ==> PUS(f)”));
 
-
-(*model is a R:A~>A with a member of Pow(A * N)
-
-type of model: Pow(A * A) * Pow(A * N)
- *)
-
-val Vof_def = qdefine_fsym("Vof",[‘M:mem(Pow(W * W) * Exp(W,Pow(A)))’])
-‘tof(Snd(M))’ |> gen_all
-
-
-val Rof_def = qdefine_fsym("Rof",[‘M:mem(Pow(W * W) * Exp(W,Pow(A)))’])
-‘Fst(M)’ |> gen_all
-
-
-val satis_cheat = 
-    qdefine_psym("satis",
-                 [‘M:mem(Pow(W * W) * Exp(W,Pow(A)))’,‘w:mem(W)’,‘f:mem(form(A))’])
-    ‘T’
-
-
-(*related*)
-val Rlt_def = qdefine_psym("Rlt",[‘M:mem(Pow(W * W) * Exp(W,Pow(A)))’,‘w1:mem(W)’,‘w2:mem(W)’]) ‘IN(Pair(w1,w2),Rof(M))’
-
-val Sim_def = qdefine_psym("Sim",[‘R:W1~>W2’,‘M1:mem(Pow(W1 * W1) * Exp(W1,Pow(A)))’,‘M2:mem(Pow(W2 * W2) * Exp(W2,Pow(A)))’]) 
-‘!w1 w2.Holds(R,w1,w2) ==>
- (!p.IN(p,App(Vof(M1),w1)) ==> IN(p,App(Vof(M2),w2))) & 
- (!v. Rm(M1,w1,v) ==> ?v'. Holds(R,v,v') & Rm(M2,w2,v'))’
-
-val PUS_def = qdefine_psym("PUS",[‘f:mem(form(A))’])
-‘!W1 W2 R:W1~>W2 M1:mem(Pow(W1 * W1) * Exp(W1,Pow(A))) M2. Sim(R,M1,M2) ==>
- !w1 w2. Holds(R,w1,w2) ==> satis(M1,w1,f) ==> satis(M2,w2,f)’
-
-val PE_cheat = qdefine_psym("PE",[‘f:mem(form(A))’]) ‘T’
-
-val EQV_def = qdefine_psym("EQV",[‘f1:mem(form(A))’,‘f2:mem(form(A))’])
- ‘!W M w:mem(W). satis(M,w,f1) <=> satis(M,w,f2)’
 
 val Sab_def = qdefine_psym
                   ("Sab",[‘fs:mem(Pow(form(A)))’,‘X:mem(Pow(W))’,‘M:mem(Pow(W * W) * Exp(W,Pow(A)))’])
@@ -905,54 +1004,11 @@ cheat
 val Msat_def = qdefine_psym("Msat",[‘M:mem(Pow(W * W) * Exp(W,Pow(A)))’]) 
 ‘!w fs. Fsab(fs,Sucm(M,w),M) ==>  Sab(fs,Sucm(M,w),M) ’
 
-val INTER_def = proved_th $ 
-e0
-cheat
-(form_goal “!A. ?f:Pow(A) * Pow(A) -> Pow(A).
- !s1 s2 a. IN(a,App(f,Pair(s1,s2))) <=> IN(a,s1) & IN(a,s2)”)
-|> spec_all |> qSKOLEM "INTER" [‘A’]
-
-val Inter_def = qdefine_fsym("Inter",[‘s1:mem(Pow(A))’,‘s2:mem(Pow(A))’])
-‘App(INTER(A),Pair(s1,s2))’
-
-
-
-val UNION_def = proved_th $ 
-e0
-cheat
-(form_goal “!A. ?f:Pow(A) * Pow(A) -> Pow(A).
- !s1 s2 a. IN(a,App(f,Pair(s1,s2))) <=> IN(a,s1) | IN(a,s2)”)
-|> spec_all |> qSKOLEM "UNION" [‘A’]
-
-val IN_Inter = prove_store("IN_Inter",
-e0
-cheat
-(form_goal “!A s1 s2 a. IN(a:mem(A),Inter(s1,s2)) <=> IN(a,s1) & IN(a,s2)”));
-
-val EMPTY_def = qdefine_psym("EMPTY",[‘A’])
-‘!x:mem(A).F’
-
 val filter_def = qdefine_psym("filter",[‘L:mem(Pow(Pow(J)))’,‘J’])
 ‘~EMPTY(J) &
   ~(L = Empty(Pow(J))) & IN(Whole(J),L) & 
   (!X Y. IN(X,L) & IN(Y,L) ==> IN(Inter(X,Y),L)) & 
   (!X. IN(X,L) ==> !Y. SS(X,Y) ==> IN(Y,L))’
-
-
-val COMPL_def = proved_th $ 
-e0
-cheat
-(form_goal “!A. ?f:Pow(A) -> Pow(A).
- !s a. IN(a,App(f,s)) <=> ~IN(a,s)”)
-|> spec_all |> qSKOLEM "COMPL" [‘A’]
-
-val Compl_def = qdefine_fsym("Compl",[‘s:mem(Pow(A))’])
-‘App(COMPL(A),s)’
-
-val IN_Compl = prove_store("IN_Compl",
-e0
-cheat
-(form_goal “!A s a. IN(a:mem(A),Compl(s)) <=> ~IN(a,s)”));
 
 
 val ufilter_def = qdefine_psym("ufilter",[‘L:mem(Pow(Pow(J)))’,‘J’])
@@ -1063,7 +1119,7 @@ val Prop_5_8 = prove_store("Prop_5_8",
 e0
 (strip_tac >> strip_tac >> strip_tac >>
  ind_with (form_induct |> qspecl [‘A’]) >>
- rpt strip_tac >-- cheat >-- cheat >-- cheat >-- cheat >>
+ rpt strip_tac >-- cheat >-- cheat >-- cheat >-- cheat >> cheat
  )
 (form_goal “!W M:mem(Pow(W * W) * Exp(W,Pow(A))) u phi.
  IN(Sw(M,phi),Repu(u)) <=> satis(UE(M),u,phi) ”));
@@ -1154,7 +1210,7 @@ e0
 
 val Prop_5_9 = prove_store("Prop_5_9",
 e0
-(strip_tac >> rw[Msat_def] >> rpt strip_tac >>
+(cheat(*strip_tac >> rw[Msat_def] >> rpt strip_tac >>
  qcases ‘EMPTY(W)’ >-- cheat >>
  qby_tac
  ‘?D0. !ws. IN(ws,D0) <=>
@@ -1214,7 +1270,7 @@ cheat >>
  qexists_tac ‘Sing(f)’ >> rw[Fin_Sing] >>
  arw[SS_def,Sing_def,Sg_def] >>
  rpt strip_tac >-- arw[] >>
- rw[Sw_def,SW_def,GSYM Sing_def,SATIS_Sing])
+ rw[Sw_def,SW_def,GSYM Sing_def,SATIS_Sing] *))
 (form_goal “!M:mem(Pow(W * W) * Exp(W,Pow(A))). Msat(UE(M))”));
 
 
@@ -1225,6 +1281,11 @@ cheat
 (form_goal “!M1 M2.Msat(M1) & Msat(M2) ==> 
  !w1:mem(W1) w2:mem(W2). (!f:mem(form(A)).PE(f) ==> satis(M1,w1,f) ==> satis(M2,w2,f)) ==>
  ?R. Sim(R,M1,M2) & Holds(R,w1,w2)”));
+
+
+val SATIS_def = qdefine_psym("SATIS",
+[‘M:mem(Pow(W * W) * Exp(W,Pow(A)))’,‘w:mem(W)’,‘fs:mem(Pow(form(A)))’])
+‘!f. IN(f,fs) ==> satis(M,w,f)’
 
 val Thm_6_23 = prove_store("Thm_6_23",
 e0
@@ -1237,9 +1298,6 @@ cheat
   ?W M:mem(Pow(W * W) * Exp(W,Pow(A))) w. 
    SATIS(M,w,fs) ”));
 
-val SATIS_def = qdefine_psym("SATIS",
-[‘M:mem(Pow(W * W) * Exp(W,Pow(A)))’,‘w:mem(W)’,‘fs:mem(Pow(form(A)))’])
-‘!f. IN(f,fs) ==> satis(M,w,f)’
 
 
 val ENT_def = qdefine_psym("ENT",[‘phis:mem(Pow(form(A)))’,‘psi:mem(form(A))’])
@@ -1287,16 +1345,16 @@ cheat
 (form_goal “!f M:mem(Pow(W * W) * Exp(W,Pow(A))) w.
  satis(M,w,f) ==> SATIS(M,w,PEC(f)) ”));
 
-val satis_NEG = prove_store("satis_NEG",
+val satis_Neg = prove_store("satis_Neg",
 e0
 cheat
 (form_goal
- “!M:mem(Pow(W * W) * Exp(W,Pow(A))) w.satis(M, w, NEG(f)) <=> ~satis(M, w, f)”));
+ “!M:mem(Pow(W * W) * Exp(W,Pow(A))) w.satis(M, w, Neg(f)) <=> ~satis(M, w, f)”));
 
-val NEG_eq_eq = prove_store("NEG_eq_eq",
+val Neg_eq_eq = prove_store("Neg_eq_eq",
 e0
 cheat
-(form_goal “!f1:mem(form(A)) f2.NEG(f1) = NEG(f2) <=> f1 = f2”));
+(form_goal “!f1:mem(form(A)) f2.Neg(f1) = Neg(f2) <=> f1 = f2”));
 
 
 val Thm_6_25_l2r = prove_store("Thm_6_25_l2r",
@@ -1320,10 +1378,10 @@ e0
      fs[ENT_def]) >>
  rw[ENT_def] >> rpt strip_tac >>
  qby_tac
- ‘?G. !psi. IN(psi,G) <=>?psi0. psi = NEG(psi0) & PE(psi0) & ~(satis(M,w,psi0))’
+ ‘?G. !psi. IN(psi,G) <=>?psi0. psi = Neg(psi0) & PE(psi0) & ~(satis(M,w,psi0))’
  >-- accept_tac (IN_def_P |> qspecl [‘form(A)’]
               |> fVar_sInst_th “P(psi:mem(form(A)))”
-                 “?psi0:mem(form(A)). psi = NEG(psi0) & PE(psi0) & 
+                 “?psi0:mem(form(A)). psi = Neg(psi0) & PE(psi0) & 
                                       ~(satis(M,w:mem(W),psi0))”
               |> uex2ex_rule) >>
  pop_assum strip_assume_tac >>
@@ -1333,16 +1391,16 @@ e0
  >-- (rpt strip_tac >> ccontra_tac >>
      qby_tac
      ‘?ss0. !f0. IN(f0,ss0) <=> 
-      IN(NEG(f0),Del(ss,f))’ 
+      IN(Neg(f0),Del(ss,f))’ 
      >-- accept_tac (IN_def_P |> qspecl [‘form(A)’]
               |> fVar_sInst_th “P(f0:mem(form(A)))”
-                 “IN(NEG(f0),Del(ss,f:mem(form(A))))”
+                 “IN(Neg(f0),Del(ss,f:mem(form(A))))”
               |> uex2ex_rule) >> 
      pop_assum strip_assume_tac >>
      qby_tac ‘Fin(ss0)’ >-- (*FINITE_Inj*) cheat >>
      qby_tac
-     ‘!psi0.IN(NEG(psi0),G) ==> PE(psi0) & ~satis(M,w,psi0)’
-     >-- (arw[] >> rw[NEG_eq_eq] >> rpt strip_tac >> rfs[] >> arw[]) >>
+     ‘!psi0.IN(Neg(psi0),G) ==> PE(psi0) & ~satis(M,w,psi0)’
+     >-- (arw[] >> rw[Neg_eq_eq] >> rpt strip_tac >> rfs[] >> arw[]) >>
      qby_tac ‘SS(Del(ss,f),G)’ >-- cheat >> 
      qby_tac ‘!f0. IN(f0,ss0) ==> PE(f0)’ 
      >-- (rpt strip_tac >> drule $ iffLR SS_def >> 
@@ -1362,10 +1420,10 @@ e0
           qexistsl_tac [‘W'’,‘M'’,‘w'’] >>
           qby_tac ‘!f1. IN(f1,Del(ss,f)) ==> satis(M',w',f1)’ 
           >-- (rpt strip_tac >>
-              qby_tac ‘?f0. f1 = NEG(f0)’ >-- cheat >> fs[] >>
+              qby_tac ‘?f0. f1 = Neg(f0)’ >-- cheat >> fs[] >>
               fs[] >> ccontra_tac  >>
-              qby_tac ‘?f0. IN(NEG(f0),Del(ss,f)) & satis(M',w',f0)’ 
-              >-- (qexists_tac ‘f0’ >> arw[] >> fs[satis_NEG]) >>
+              qby_tac ‘?f0. IN(Neg(f0),Del(ss,f)) & satis(M',w',f0)’ 
+              >-- (qexists_tac ‘f0’ >> arw[] >> fs[satis_Neg]) >>
               first_x_assum opposite_tac) >>
           rw[SATIS_def] >> rpt strip_tac >>
           qcases ‘f' = f’ 
@@ -1381,13 +1439,13 @@ e0
      qby_tac ‘!f0.IN(f0,ss0) ==> ~satis(M,w,f0)’ 
      >-- (rpt strip_tac >> 
          last_x_assum $ drule o iffLR >> 
-         qby_tac ‘IN(NEG(f0'),G)’
+         qby_tac ‘IN(Neg(f0'),G)’
          >-- (qsuff_tac ‘SS(Del(ss,f),G)’
              >-- (rw[SS_def] >> rpt strip_tac >>
                  first_x_assum irule >> arw[]) >>
              cheat (* SS(ss, Ins(f, G)) ==> SS(Del(ss, f), G)*)) >>
          pop_assum mp_tac >> arw[] >> strip_tac >>
-         fs[NEG_eq_eq]) >>
+         fs[Neg_eq_eq]) >>
      first_x_assum drule >> fs[])>>
  drule Thm_6_23 >> pop_assum strip_assume_tac >>
  qby_tac ‘!psi. PE(psi) ==> satis(M',w',psi) ==> satis(M,w,psi)’ 
@@ -1395,12 +1453,12 @@ e0
      >-- (rpt strip_tac >> ccontra_tac >> 
          first_x_assum drule >> first_x_assum drule >> fs[]) >>
      rpt strip_tac >>
-     qby_tac ‘IN(NEG(psi),G)’ 
+     qby_tac ‘IN(Neg(psi),G)’ 
      >-- (first_x_assum (irule o iffRL) >>
          qexists_tac ‘psi’ >> arw[]) >> 
      drule $ iffLR SATIS_def >>
-     first_x_assum (qsspecl_then [‘NEG(psi)’] assume_tac) >>
-     rfs[Ins_def,satis_NEG]) >>
+     first_x_assum (qsspecl_then [‘Neg(psi)’] assume_tac) >>
+     rfs[Ins_def,satis_Neg]) >>
  qby_tac
  ‘?R. Sim(R,UE(M'),UE(M)) & Holds(R,Pft(w'),Pft(w))’
  >-- (irule Thm_6_22 >> rw[Prop_5_9] >> rpt strip_tac >>
